Chorlean.lean
@@ -1,5 +1,3 @@
 -- This module serves as the root of the `Chorlean` library.
 -- Import modules here that should be built as part of the library.
 import «Chorlean».Basic
-
-def TEST_DEF := 2
