README.md
@@ -1,3 +1,102 @@
-# chorlean
+# ChorLean
 
 Implementation of choreographic library based programming in the style of HasChor/MultiChor
+
+## Usage
+
+### Roles
+
+First, a Choreo requires an instance of the *Role* class.
+*Role* specifies how many entities participate in the choreography and gives them unique string identifiers.
+These identifiers are used for debugging information, and to select which role to execute when running choreographies on the command line.
+Optionally, the *adj* (adjacency) field can specify which roles are allowed to communicate with which other role. 
+By default, there are no restrictions on adjacency between roles.
+
+#### Buyer-Seller Roles
+
+Here is an example Role instance taken from the bookseller example:
+```lean
+instance: Role where
+  N := 2
+  name | 0 => "buyer" | 1 => "seller"
+```
+
+### Executing Endpoint
+Choreographic code is always executed by a single role that runs those instructions relevant to them.
+This role is an argument for running choreographies, and usually passed by the user when starting the program on the command line.
+Programmers do not have direct access to the endpoint, but only through the libraries API.
+This role is called *ep* for endpoint.
+
+### Choreo Monad
+
+Choreographies in ChorLean are written in the *Choreo* Monad.
+*Choreo* is parameterized by:
+- the set of roles that participate in that function (present roles), all other roles will ignore that code. The set is specified as a predicate over roles, where all roles fulfilling that predicate participate 
+- Evidence that the endpoint fulfills the predicate
+
+### Main Entrypoint
+Chorlean provides a function that automatically generates the main function for you, called *CHOR_ENTRYPOINT*, and a main function is expected to be defined as:
+```lean
+def main := CHOR_ENTRYPOINT
+```
+CHOR_ENTRYPOINT lets you run the choreography by running the Lean program and supplying the *Role.name* as the first command line argument.
+CHOR_ENTRYPOINT expects an instance of the *ChorMain* class, containing the actual Main method.
+The Main method maps the command line inputs as a faceted list of strings, to a choreography that initially contains *all* roles.
+
+### Located Values and Types
+
+Types in ChorLean are annotated by which roles have knowledge of them by predicates (similar to present roles).
+They are notated as *α @ p* where *α* is a type and *p* a predicate over roles.
+Located values are defined as functions from evidence, that the endpoint has knowledge of the value (fulfills the predicate), to the value itself. Such evidence can be gathered by *enclaving*.
+Helpful functions around located values include:
+
+- Located.wrap: wraps values into located values
+- Located.flatten: removes one layer of nested located values
+- Located.cast: casts into a located value with different predicate *p'*, if *(p x -> p' x)*. This is also helpful when two propositions describe the same set of roles, like *x ∈ [A]* and *x=A*
+
+#### Faceted
+Maps roles to located values which are located at them. Helpful for parallel computations.
+
+### Basic Operations
+
+The Core of ChorLean is built on only 3 functions
+
+1. Enclave: embeds a choreography containing less present roles into a bigger one.
+2. Broadcast: broadcasts a located value to all present roles, such that it can then be used as a non-located value.
+3. Locally: runs a program on the present role. *Requires* a single location to be present.
+
+### Other helpful functions and notations:
+
+#### Enclaves
+
+The examples make use the following notation for enclave: *a ~ b* and *a ° b*, where *a* is something with a membership relation (like lists) and *b* is the subchoreography to enclave. Using the *°*, the result of the enclave is also broadcasted. By *[A]° locally IO.getLine* the Role A would perform a getline program locally and broadcast it afterwards.
+
+#### Parallel
+
+Iterates over all present roles to perform a program locally on them. The program in this case has knowledge of the identity of the executing role. Results in *faceted* values. A Choreography where every role prints their identity looks like this
+```lean
+par fun id => IO.println s!"hello from {id}"
+```
+
+#### Scatter/Gather
+
+A sender can scatter data located at him by sending every present role a value of the same type, resulting in a faceted value. To inverse this, a faceted value can be gathered in a single location again.
+Additionally, there is a *scatterList* and *gatherList* variant, which scatters and gathers list items evenly. *gatherAll* is a variant of gather that gathers results replicated at all roles, not just a single one.
+
+## Examples
+run the examples by:
+```
+booseller:
+lake exe books buyer
+lake exe books seller
+
+authentication:
+lake exe auth client
+lake exe auth service
+lake exe auth IP
+
+mergesort:
+lake exe merge master
+lake exe merge W1
+lake exe merge W2
+```
